

$$\phi - \phi_0 = \int_{r_0}^r \frac{L}{r^2 \sqrt{2\mu[-U(r)] - \frac{L^2}{r^2}}} dr$$

For  $\mu = 0$  :  $U(r) = -\frac{\nu r^2}{2r^2}$

Let  $u = \frac{1}{r}$   $U(u) = -\frac{\nu r^2 u^2}{2}$

$du = -r^{-2}$

$$\phi - \phi_0 = \int_{\frac{1}{r_0}}^{\frac{1}{r}} \frac{L}{\sqrt{2\mu \nu r^2 u^2 - L^2 u^2}} du$$

$$\phi - \phi_0 = \int_{u_0}^u \frac{L}{u \sqrt{\mu \nu r^2 - L^2}} du$$

$$\phi - \phi_0 = \frac{L}{\sqrt{\mu \nu r^2 - L^2}} \int_{u_0}^u \frac{1}{u} du$$

$$\phi - \phi_0 = \frac{L}{\sqrt{\mu \nu r^2 - L^2}} \left[ \ln\left(\frac{1}{u}\right) - \ln\left(\frac{1}{u_0}\right) \right]$$

Let  $u = \frac{1}{r}$

$$\phi - \phi_0 = \frac{L}{\sqrt{\mu \nu r^2 - L^2}} \ln\left(\frac{r}{r_0}\right)$$

Let  $\phi_0 = 0$  :  $\phi = \frac{L}{\sqrt{\mu \nu r^2 - L^2}} \ln\left(\frac{r}{r_0}\right)$

Notes:

~~$\frac{1}{r} = A \cos \theta + \frac{1}{r}$~~

~~$\frac{1}{r} = \frac{1}{A} \cos \theta + \frac{1}{r}$~~

~~$\ln\left(\frac{1}{A r}\right) = \ln \theta + \frac{1}{r}$~~

~~$\ln\left(\frac{1}{A r}\right) = \ln \theta + \frac{1}{r}$~~

~~$\theta = \frac{1}{r}$~~